exercises/chapter05-distributed-state-machines/exercise03.dfy
@@ -16,14 +16,80 @@ module TwoPCInvariantProof {
     requires v.WF()
   {
     // FIXME: fill in here (solution: 5 lines)
-     true // Replace me
-    // END EDIT
+    && (forall m: Message | m in v.network.sentMsgs && m.MsgDecison?
+          :: && CoordinatorVars(v).decision.Some?
+             && m.d == CoordinatorVars(v).decision.value)
+    && (forall m: Message, i: HostId |
+          && m in v.network.sentMsgs
+          && m.MsgDecison?
+          && ValidParticipantId(v, i)
+          && ParticipantVars(v, i).decision.Some?
+          :: (m.d == ParticipantVars(v, i).decision.value))
+       // END EDIT
   }
 
   // We use this block of code to define additional invariants. We recommend you
   // define predicates for the individual parts of your invariant, to make
   // debugging easier.
   // FIXME: fill in here (solution: 20 lines)
+  ghost predicate ParticipantDecideAfterCoordinator(v: Variables)
+    requires v.WF()
+  {
+    CoordinatorVars(v).decision.None? ==> forall i: HostId | ValidParticipantId(v, i)
+        :: ParticipantVars(v, i).decision.None?
+  }
+
+  // ghost predicate VoteAgreeWithPreference(v: Variables)
+  //   requires v.WF()
+  // {
+  //   forall i: HostId | ValidParticipantId(v, i)
+  //     :: && var pref := ParticipantVars(v, i).c.preference;
+  //        && var vote := CoordinatorVars(v).votes[i];
+  //        && (vote.Some? ==> (vote.value == pref))
+  // }
+
+  // ghost predicate VoteMsgAgreeWithPreference(v: Variables)
+  //   requires v.WF()
+  // {
+  //   forall i: HostId, m: Message |
+  //     && ValidParticipantId(v, i)
+  //     && m in v.network.sentMsgs
+  //     && m.MsgVote?
+  //     && m.p == i
+  //     :: && var pref := ParticipantVars(v, i).c.preference;
+  //        && var vote := CoordinatorVars(v).votes[i];
+  //        && m.vote == pref
+  //        && (vote.Some? ==> (vote.value == pref))
+  // }
+
+  ghost predicate RecvVoteImpliesVoteMsgSent(v: Variables)
+    requires v.WF()
+  {
+    forall i: HostId | ValidParticipantId(v, i)
+      :: CoordinatorVars(v).votes[i].Some? ==> (
+             exists m: Message ::
+               && m in v.network.sentMsgs
+               && m.MsgVote?
+               && m.p == i
+               && m.vote == CoordinatorVars(v).votes[i].value
+           )
+  }
+
+  ghost predicate VoteMsgImpliesPreference(v: Variables)
+    requires v.WF()
+  {
+    forall i: HostId | ValidParticipantId(v, i)
+      :: (exists m: Message ::
+            && m in v.network.sentMsgs
+            && m.MsgVote?
+            && m.p == i) ==> (
+             forall m: Message | && m in v.network.sentMsgs
+                                 && m.MsgVote?
+                                 && m.p == i
+               :: m.vote == ParticipantVars(v, i).c.preference
+           )
+  }
+
   // END EDIT
 
 
@@ -34,6 +100,10 @@ module TwoPCInvariantProof {
        // END EDIT
        // We give you the blueprint for one invariant to get you started...
     && DecisionMsgsAgreeWithDecision(v)
+    && ParticipantDecideAfterCoordinator(v)
+    && RecvVoteImpliesVoteMsgSent(v)
+    && VoteMsgImpliesPreference(v)
+       // && VoteAgreeWithPreference(v)
        // ...but you'll need more.
     && Safety(v)
   }
@@ -43,6 +113,7 @@ module TwoPCInvariantProof {
     ensures Inv(v)
   {
     // FIXME: fill in here (solution: 3 lines)
+    assert !CoordinatorVars(v).decision.Some?;
     // END EDIT
   }
 
@@ -53,6 +124,226 @@ module TwoPCInvariantProof {
   {
     //(not all of the below but much of it)
     // FIXME: fill in here (solution: 59 lines)
+    var step :| NextStep(v, v', step);
+    var hostId := step.hostId;
+    var msgOps := step.msgOps;
+
+    var cv := CoordinatorVars(v);
+    var cv' := CoordinatorVars(v');
+
+    if ValidParticipantId(v, hostId) {
+      var pv := ParticipantVars(v, hostId);
+      var pv' := ParticipantVars(v', hostId);
+      var hostStep :| ParticipantHost.NextStep(pv, pv', hostStep, msgOps);
+      if msgOps.recv.Some? && msgOps.send.Some? {
+        assert hostStep.CastVoteStep?;
+        assert forall i: HostId | ValidParticipantId(v, i)
+            :: ParticipantVars(v, i) == ParticipantVars(v', i);
+        assert SafetyAC1(v');
+        assert SafetyAC3(v');
+        assert SafetyAC4(v');
+        assert VoteMsgImpliesPreference(v');
+      } else if msgOps.recv.Some? && msgOps.send.None? {
+        var m := msgOps.recv.value;
+        assert m.MsgDecison?;
+        assert hostStep.AcceptDecisionStep?;
+        assert ParticipantHost.AcceptDecision(pv, pv', msgOps);
+
+        {
+          forall i: HostId, j: HostId |
+            && ValidParticipantId(v', i)
+            && ValidParticipantId(v', j)
+            && ParticipantVars(v', i).decision.Some?
+            && ParticipantVars(v', j).decision.Some?
+            ensures ParticipantVars(v', i).decision.value == ParticipantVars(v', j).decision.value
+          {
+            var di' := ParticipantVars(v', i).decision.value;
+            var dj' := ParticipantVars(v', j).decision.value;
+
+            assert (forall m: Message | m in v'.network.sentMsgs && m.MsgDecison?
+                      :: && CoordinatorVars(v').decision.Some?
+                         && m.d == CoordinatorVars(v').decision.value);
+            forall m_: Message, i: HostId |
+              && m_ in v'.network.sentMsgs
+              && m_.MsgDecison?
+              && ValidParticipantId(v', i)
+              && ParticipantVars(v', i).decision.Some?
+              ensures (m_.d == ParticipantVars(v', i).decision.value) {
+              assert m_ in v'.network.sentMsgs;
+              if i != hostId {
+                assert m_.d == ParticipantVars(v, i).decision.value;
+                assert ParticipantVars(v, i).decision == ParticipantVars(v', i).decision;
+              } else {
+                assert ParticipantVars(v', i).decision.Some? && ParticipantVars(v', i).decision.value == m.d;
+              }
+            }
+            assert DecisionMsgsAgreeWithDecision(v');
+            assert di' == m.d;
+            assert dj' == m.d;
+            assert di' == dj';
+          }
+          assert SafetyAC1(v');
+        }
+
+        {
+          if exists i: HostId :: ValidParticipantId(v', i) && ParticipantVars(v', i).c.preference == No {
+            var i: HostId :| ValidParticipantId(v', i) && ParticipantVars(v', i).c.preference == No;
+            assert ParticipantVars(v, i).c.preference == No;
+            if CoordinatorVars(v').decision.Some? {
+              assert cv.decision == cv'.decision;
+              assert cv'.decision.value == Abort;
+            }
+          }
+          assert SafetyAC3(v');
+        }
+
+        {
+          if forall i: HostId | ValidParticipantId(v', i) :: ParticipantVars(v', i).c.preference == Yes
+          {
+            assert SafetyAC4(v);
+            assert forall i: HostId :: ValidParticipantId(v, i) == ValidParticipantId(v', i);
+            assert forall i: HostId | ValidParticipantId(v, i) :: ParticipantVars(v, i).c.preference == Yes;
+            assert CoordinatorVars(v).decision.Some? ==> (CoordinatorVars(v).decision.value == Commit);
+            assert cv' == cv;
+            assert cv.decision.Some? ==> (cv.decision.value == Commit);
+            assert cv'.decision.Some? ==> (cv'.decision.value == Commit);
+          }
+          assert (forall i: HostId | ValidParticipantId(v', i) :: ParticipantVars(v', i).c.preference == Yes)
+            ==> (forall i: HostId | ValidParticipantId(v', i)
+                   :: (ParticipantVars(v', i).decision.Some? ==> ParticipantVars(v', i).decision.value == Commit)
+              );
+          assert SafetyAC4(v');
+        }
+
+        {
+          forall i: HostId, m: Message |
+            && ValidParticipantId(v', i)
+            && m in v'.network.sentMsgs
+            && m.MsgVote?
+            && m.p == i
+            ensures m.vote == ParticipantVars(v', i).c.preference {
+            assert v.network.sentMsgs == v'.network.sentMsgs;
+            assert ParticipantVars(v, i).c.preference == ParticipantVars(v', i).c.preference;
+          }
+          assert VoteMsgImpliesPreference(v');
+        }
+      } else if msgOps.recv.None? && msgOps.send.Some? {
+        assert false;
+      } else { // msgOps.recv.None? && msgOps.send.None?
+        assert false;
+      }
+    } else if ValidCoordinatorId(v, hostId) { // must be coordinator
+      var hostStep :| CoordinatorHost.NextStep(cv, cv', hostStep, msgOps);
+      if msgOps.recv.Some? && msgOps.send.Some? {
+        assert false;
+      } else if msgOps.recv.Some? && msgOps.send.None? {
+        var m := msgOps.recv.value;
+        assert m.MsgVote?;
+        assert hostStep.RecvVoteStep?;
+        assert cv.decision == cv'.decision;
+        assert forall i | ValidParticipantId(v, i) :: ParticipantVars(v, i) == ParticipantVars(v', i);
+        assert SafetyAC1(v');
+        assert SafetyAC3(v');
+        assert SafetyAC4(v');
+        assert VoteMsgImpliesPreference(v');
+      } else if msgOps.recv.None? && msgOps.send.Some? {
+        var m := msgOps.send.value;
+        match m {
+          case MsgReqVote => {
+            var hostStep :| CoordinatorHost.NextStep(cv, cv', hostStep, msgOps);
+            assert hostStep.ReqVoteStep?;
+            assert CoordinatorHost.ReqVote(cv, cv', msgOps);
+            assert cv == cv';
+            assert forall i | ValidParticipantId(v, i) :: ParticipantVars(v, i) == ParticipantVars(v', i);
+            assert SafetyAC1(v');
+            assert SafetyAC3(v');
+            assert SafetyAC4(v');
+            assert VoteMsgImpliesPreference(v');
+          }
+          case MsgDecison(d) => {
+            var hostStep :| CoordinatorHost.NextStep(cv, cv', hostStep, msgOps);
+            assert hostStep.DecideAndSendStep?;
+            assert CoordinatorHost.DecideAndSend(cv, cv', msgOps);
+
+            {
+              assert forall i: HostId | ValidParticipantId(v, i)
+                  :: ParticipantVars(v, i).decision == ParticipantVars(v', i).decision;
+              assert (forall i: HostId, j: HostId |
+                        && ValidParticipantId(v', i)
+                        && ValidParticipantId(v', j)
+                        && ParticipantVars(v', i).decision.Some?
+                        && ParticipantVars(v', j).decision.Some?
+                        :: ParticipantVars(v', i).decision.value == ParticipantVars(v', j).decision.value);
+
+              assert forall i: HostId | ValidParticipantId(v, i)
+                  :: ParticipantVars(v, i).decision.None?;
+              assert (forall i: HostId |
+                        && ValidParticipantId(v', i)
+                        && ParticipantVars(v', i).decision.Some?
+                        && CoordinatorVars(v').decision.Some?
+                        :: ParticipantVars(v', i).decision.value == CoordinatorVars(v').decision.value);
+              assert SafetyAC1(v');
+            }
+
+            {
+              if exists i: HostId :: ValidParticipantId(v', i) && ParticipantVars(v', i).c.preference == No {
+                var i: HostId :| ValidParticipantId(v', i) && ParticipantVars(v', i).c.preference == No;
+                assert cv'.votes[i].Some?;
+                assert RecvVoteImpliesVoteMsgSent(v');
+                assert forall m: Message | m in v'.network.sentMsgs && m.MsgVote? && m.p == i
+                    :: m.vote == CoordinatorVars(v').votes[i].value;
+                assert VoteMsgImpliesPreference(v');
+                assert cv'.votes[i].value == No;
+                assert m.d == Abort;
+                assert cv'.decision.Some? && cv'.decision.value == Abort;
+              }
+              assert SafetyAC3(v');
+            }
+
+            {
+              if forall i: HostId | ValidParticipantId(v', i) :: ParticipantVars(v', i).c.preference == Yes {
+                var i: HostId :| ValidParticipantId(v', i);
+                if CoordinatorVars(v').decision.Some? {
+                  assert RecvVoteImpliesVoteMsgSent(v');
+                  assert exists m: Message ::
+                      && m in v'.network.sentMsgs
+                      && m.MsgVote?
+                      && m.p == i
+                      && m.vote == CoordinatorVars(v').votes[i].value;
+                  assert VoteMsgImpliesPreference(v');
+                  assert forall m: Message | && m in v'.network.sentMsgs
+                                             && m.MsgVote?
+                                             && m.p == i
+                      :: m.vote == ParticipantVars(v', i).c.preference;
+                  assert CoordinatorVars(v').decision.value == Commit;
+                }
+              }
+
+              assert (forall i: HostId | ValidParticipantId(v', i) :: ParticipantVars(v', i).c.preference == Yes)
+                ==> (forall i: HostId | ValidParticipantId(v', i)
+                       :: (ParticipantVars(v', i).decision.Some? ==> (ParticipantVars(v', i).decision.value == Commit))
+                  );
+              assert SafetyAC4(v');
+            }
+            assert VoteMsgImpliesPreference(v');
+          }
+          case _ => assert false;
+        }
+        assert SafetyAC1(v');
+        assert SafetyAC3(v');
+        assert SafetyAC4(v');
+      } else { // msgOps.recv.None? && msgOps.send.None?
+        assert false;
+      }
+    } else {
+      assert false;
+    }
+
+    assert SafetyAC1(v');
+    assert SafetyAC3(v');
+    assert SafetyAC4(v');
+    assert RecvVoteImpliesVoteMsgSent(v');
+    assert VoteMsgImpliesPreference(v');
     // END EDIT
   }
 
